Instances/ISAs/VexBridgeCore.lean
@@ -42,7 +42,7 @@ def BridgeInvariant {Reg : Type} [DecidableEq Reg] [Fintype Reg]
     (input : ConcreteState Reg)
     (concrete : ConcreteState Reg × TempEnv) (sub : SymSub Reg) (temps : SymTempEnv Reg) : Prop :=
   concrete.1 = applySymSub sub input ∧
-    ∀ tmp, concrete.2 tmp = evalSymExpr input (temps tmp)
+    ∀ tmp, concrete.2 tmp = evalSymExpr input (temps.get tmp)
 
 abbrev LowerStateMatches {Reg : Type} [DecidableEq Reg] [Fintype Reg]
     (input : ConcreteState Reg)
@@ -98,7 +98,7 @@ structure BranchStmtBridgeCase {Reg : Type} [DecidableEq Reg] [Fintype Reg]
 private theorem lowerExpr_sound {Reg : Type} [DecidableEq Reg] [Fintype Reg]
     (input state : ConcreteState Reg) (temps : TempEnv) (sub : SymSub Reg) (symTemps : SymTempEnv Reg)
     (hState : state = applySymSub sub input)
-    (hTemps : ∀ tmp, temps tmp = evalSymExpr input (symTemps tmp))
+    (hTemps : ∀ tmp, temps tmp = evalSymExpr input (symTemps.get tmp))
     (expr : Expr Reg) :
     evalExpr state temps expr = evalSymExpr input (lowerExpr sub symTemps expr) := by
   induction expr with
@@ -106,7 +106,7 @@ private theorem lowerExpr_sound {Reg : Type} [DecidableEq Reg] [Fintype Reg]
   | get reg =>
       rw [hState]
       simpa [lowerExpr] using ConcreteState.read_applySymSub sub input reg
-  | tmp tmp => simp [lowerExpr, hTemps]
+  | tmp tmp => simp [lowerExpr, SymTempEnv.get, hTemps]
   | narrow32 expr ih =>
       simp only [evalExpr, lowerExpr, foldUn]; split <;> simp_all [evalSymExpr, mask32]
   | zext64 expr ih =>
@@ -161,7 +161,7 @@ private theorem lowerExpr_sound {Reg : Type} [DecidableEq Reg] [Fintype Reg]
 private theorem lowerCond_sound {Reg : Type} [DecidableEq Reg] [Fintype Reg]
     (input state : ConcreteState Reg) (temps : TempEnv) (sub : SymSub Reg) (symTemps : SymTempEnv Reg)
     (hState : state = applySymSub sub input)
-    (hTemps : ∀ tmp, temps tmp = evalSymExpr input (symTemps tmp))
+    (hTemps : ∀ tmp, temps tmp = evalSymExpr input (symTemps.get tmp))
     (cond : Cond Reg) :
     evalCond state temps cond = evalSymPC input (lowerCond sub symTemps cond) := by
   cases cond with
@@ -226,8 +226,9 @@ private theorem applySymSub_writeMem {Reg : Type} [DecidableEq Reg] [Fintype Reg
             by_cases h : tmp' = tmp
             · subst h
               have hExpr := lowerExpr_sound input state temps sub symTemps hState hTemps expr
-              simp [hExpr]
-            · simpa [SymTempEnv.write, TempEnv.write, h] using hTemps tmp' }
+              simp [TempEnv.write, hExpr]
+            · simp [TempEnv.write, h, SymTempEnv.get_write_other _ _ h]
+              exact hTemps tmp' }
   | .put reg expr =>
       { exec := fun cfg =>
           match cfg with
